[minor] State refinement QA/C with generic table.
Still an admit left.

pico-ifc-coq/dyn_allocation/RefinementAC.v
@@ -36,7 +36,7 @@ Context {T: Type}
 Variable cblock : FaultRoutine.block.
 Hypothesis stamp_cblock : Mem.stamp cblock = Kernel.
 
-Let ctable_impl : list CSysCallImpl := nil.
+Variable ctable_impl : list CSysCallImpl.
 
 Let faultHandler := FaultRoutine.faultHandler _ QuasiAbstractMachine.fetch_rule.
 Let ctable := build_syscall_table (Z.of_nat (length faultHandler)) ctable_impl.
@@ -45,6 +45,7 @@ Context {WFCLatt: WfConcreteLattice cblock ctable T Latt CLatt}.
 
 Variable atable : ASysTable T.
 Hypothesis Hatable : parametric_asystable atable.
+Hypothesis Hctable_impl_correct : ctable_impl_correct cblock atable ctable_impl faultHandler.
 
 Definition tini_match_states := match_states cblock QuasiAbstractMachine.fetch_rule.
 
@@ -54,19 +55,13 @@ Program Definition abstract_concrete_ref :
   refinement (abstract_machine atable) tini_concrete_machine :=
   @ref_composition _ _ _
                    (abstract_quasi_abstract_ref Hatable)
-                   (quasi_abstract_concrete_ref stamp_cblock atable _ _)
+                   (quasi_abstract_concrete_ref stamp_cblock
+                                                (handler_correct_succeed _ _ _ _ _)
+                                                (handler_correct_fail _ _ _ _ _)
+                                                Hctable_impl_correct)
                    (@ac_match_initial_data _ _ _ cblock fetch_rule)
                    match_events
                    _ _.
-
-Next Obligation.
-  eapply handler_correct_succeed; eauto.
-Qed.
-
-Next Obligation.
-  eapply handler_correct_fail; eauto.
-Qed.
-
 Next Obligation.
   eauto.
 Qed.
