pico-ifc-coq/dyn_allocation/NIConcreteMachine.v
@@ -33,7 +33,7 @@ Context {T: Type}
 Variable cblock : FaultRoutine.block.
 Hypothesis stamp_cblock : Mem.stamp cblock = Kernel.
 
-Let ctable_impl : list CSysCallImpl := nil.
+Variable ctable_impl : list CSysCallImpl.
 
 Let faultHandler := FaultRoutine.faultHandler _ QuasiAbstractMachine.fetch_rule.
 Let ctable := build_syscall_table (Z.of_nat (length faultHandler)) ctable_impl.
@@ -42,18 +42,19 @@ Context {WFCLatt: WfConcreteLattice cblock ctable T Latt CLatt}.
 
 Variable atable : ASysTable T.
 Hypothesis Hatable : parametric_asystable atable.
+Hypothesis Hctable_impl_correct : ctable_impl_correct cblock atable ctable_impl faultHandler.
 Hypothesis table_syscall_lowstep : forall o, syscall_lowstep o atable.
 Hypothesis table_systable_inv : systable_inv atable.
 
 Inductive concrete_i_equiv (o : T) :
-  init_data (tini_concrete_machine cblock) -> init_data (tini_concrete_machine cblock) -> Prop :=
+  concrete_init_data -> concrete_init_data -> Prop :=
   | ci_equiv : forall ai1 ai2 ci1 ci2
                       (EQ : abstract_i_equiv o ai1 ai2)
                       (MATCH1 : ac_match_initial_data cblock QuasiAbstractMachine.fetch_rule ai1 ci1)
                       (MATCH2 : ac_match_initial_data cblock QuasiAbstractMachine.fetch_rule ai2 ci2),
                  concrete_i_equiv o ci1 ci2.
 
-Instance CMObservation : TINI.Observation (tini_concrete_machine cblock) (Event T) := {
+Instance CMObservation : TINI.Observation (tini_concrete_machine cblock ctable_impl) (Event T) := {
   out e := match e with
              | CEInt (z, t) m => EInt (z, valToLab t m)
            end;
@@ -65,16 +66,17 @@ Instance CMObservation : TINI.Observation (tini_concrete_machine cblock) (Event 
 Lemma ac_low_compatible :
   forall (o : T)
          (e1 : event (abstract_machine atable))
-         (e2 : event (tini_concrete_machine cblock)),
+         (e2 : CEvent),
     ref_match_events (@abstract_concrete_ref _ _ _ cblock stamp_cblock
+                                             ctable_impl
                                              WFCLatt
-                                             atable Hatable) e1 e2 ->
+                                             atable Hatable Hctable_impl_correct) e1 e2 ->
     (TINI.e_low o (TINI.out e1)
        <-> TINI.e_low o (@TINI.out _ _ CMObservation e2)).
 Proof.
   simpl.
   intros o [[x xl]] [[x' xt] m] H; simpl.
-  inv H. unfold pcatom_labToVal in ATOMS. simpl in *.
+  inv H. unfold pcatom_labToVal in ATOMS. simpl in ATOMS.
   destruct ATOMS as [? TAG]. subst x'.
   assert (valToLab xt m = xl) by (eapply labToVal_valToLab_id; eauto).
   subst. reflexivity.
@@ -95,20 +97,25 @@ Qed.
 Lemma ac_match_events_equiv :
   forall o e11 e12 e21 e22
          (EQ : @TINI.a_equiv (abstract_machine atable) _ _ o (E e11) (E e12))
-         (MATCH1 : ref_match_events (abstract_concrete_ref stamp_cblock Hatable) e11 e21)
-         (MATCH2 : ref_match_events (abstract_concrete_ref stamp_cblock Hatable) e12 e22),
-    @TINI.a_equiv (tini_concrete_machine cblock) _ _ o (E e21) (E e22).
+         (MATCH1 : ref_match_events (abstract_concrete_ref stamp_cblock Hatable Hctable_impl_correct) e11 e21)
+         (MATCH2 : ref_match_events (abstract_concrete_ref stamp_cblock Hatable Hctable_impl_correct) e12 e22),
+    @TINI.a_equiv (tini_concrete_machine cblock ctable_impl) _ _ o (E e21) (E e22).
 Proof.
   simpl.
   intros o [[x1 xl1]] [[x2 xl2]] [[x1' xt1] m1] [[x2' xt2] m2].
   intros.
   inv EQ; inv MATCH1; inv MATCH2;
-  unfold pcatom_labToVal in *; simpl in *;
-  try match goal with
-        | H : EInt _ = EInt _ |- _ => inv H
-      end;
+  repeat match goal with
+           | ATOMS : pcatom_labToVal _ _ _ |- _ =>
+             unfold pcatom_labToVal in ATOMS;
+             simpl in ATOMS; destruct ATOMS; subst
+           | H : TINI.out _ = TINI.out _ |- _ =>
+             simpl in H; inv H
+           | H : TINI.e_low _ _ |- _ =>
+             simpl in H
+         end;
   intuition; repeat subst;
-  constructor (solve [simpl in *; eauto;
+  constructor (solve [simpl; eauto;
                       repeat match goal with
                                | H : labToVal _ _ _ |- _ =>
                                  eapply labToVal_valToLab_id in H; eauto; rewrite H
@@ -117,7 +124,8 @@ Proof.
 Qed.
 
 Lemma ac_tini_preservation_premises :
-  tini_preservation_hypothesis (abstract_concrete_ref stamp_cblock Hatable).
+  tini_preservation_hypothesis
+    (abstract_concrete_ref stamp_cblock Hatable Hctable_impl_correct).
 Proof.
   intros o. exists o.
   split. { apply ac_low_compatible. }
@@ -129,9 +137,9 @@ Lemma concrete_noninterference :
   TINI.tini CMObservation.
 Proof.
    exact (@refinement_preserves_noninterference
-          (abstract_machine atable) (tini_concrete_machine cblock)
+          (abstract_machine atable) (tini_concrete_machine cblock ctable_impl)
           _ _ _
-          (abstract_concrete_ref stamp_cblock Hatable)
+          (abstract_concrete_ref stamp_cblock Hatable Hctable_impl_correct)
           (abstract_noninterference_short table_syscall_lowstep table_systable_inv)
           ac_tini_preservation_premises).
 Qed.
